### Cauchy-Riemann

:::{.proposition title="Holomorphic implies Cauchy-Riemann"}
If $f$ is differentiable at $z_0$, then the limit defining $f'(z_0)$ must exist when approaching from any direction.
Identify $f(z) = f(x, y)$ and write $z_0 = x+ iy$, then first consider $h\in RR$, so $h = h_1 + ih_2$ with $h_2 = 0$.
Then
\[
f'(z_0) = 
\lim_{h_1\to 0} { f(x+h_1, y) - f(x, y) \over h_1}
\da \dd{f}{x}(x, y)
.\]
Taking $h \in i\RR$ purely imaginary, so $h= ih_2$,
\[
f'(z_0)
= \lim_{ih_2\to 0} { f(x, y+h_2) - f(x, y) \over ih_2 } \da {1\over i} \dd{f}{y}(x, y)
.\]
Equating,
\[
\dd{f}{x} = {1\over i} \dd{f}{y}
,\]
and writing $f = u + iv$ and $1/i = -i$ yields
\[
\dd{f}{x} &= \dd{u}{x} + i \dd{v}{x} \\
{1\over i} \dd{f}{y} &= {1\over i} \qty{ \dd{u}{y} + i \dd{v}{y}} = \dd{v}{y} - i\dd{u}{y} 
.\]
Thus
\[
\dd{u}{x} = \dd{v}{y} \hspace{8em} \dd{u}{y} = -\dd{v}{x}
.\]
:::

:::{.proposition title="Polar Cauchy-Riemann equations"}
\[  
\frac{\partial u}{\partial r}=\frac{1}{r} \frac{\partial v}{\partial \theta} \quad \text { and } \quad \frac{1}{r} \frac{\partial u}{\partial \theta}=-\frac{\partial v}{\partial r}
.\]
:::

:::{.proof}
Setting 
\[
z = re^{i\theta} = r(\cos(\theta) + i\sin(\theta) ) = x+iy
\]
yields $x=r\cos(\theta), y=r\sin(\theta)$, one can identify
\[
x_r = \cos(\theta)&, x_\theta = -r\sin(\theta) \\
y_r = \sin(\theta)&, y_\theta = r\cos(\theta)
.\]

Now apply the chain rule:
\[
u_r 
&= u_x x_r + u_y y_r \\
&= v_y x_r -v_x y_r && \text{CR}\\
&= v_y \cos(\theta) - v_x \sin(\theta) \\
&= {1\over r}\qty{ v_y r\cos(\theta) - v_x r\sin(\theta) } \\
&= {1\over r}\qty { v_y y_\theta + v_x x_\theta} \\
&= {1\over r} v_\theta
.\]
Similarly,
\[
v_r
&= v_x x_r + v_y y_r \\
&= v_x \cos(\theta) + v_y\sin(\theta) \\
&= -u_y\cos(\theta) + u_x\sin(\theta) && \text{CR} \\
&= {1\over r}\qty{ -u_y r\cos(\theta) + u_x r\sin(\theta)} \\
&= {1\over r}\qty{ -u_y y_\theta - u_x x_0 } \\
&= -{1\over r} u_\theta
.\]

Thus
\[
\frac{\partial u}{\partial r}=\frac{1}{r} \frac{\partial v}{\partial \theta} \quad \text { and } \quad \frac{\partial v}{\partial r}=-\frac{1}{r} \frac{\partial u}{\partial \theta} \\
.\]

:::